a viable version

LogicGenerator/demo932/Interface.v
@@ -16,6 +16,7 @@ End LanguageSig.
 Module DerivedNames (Names: LanguageSig).
 Include Names.
   Definition sepcon := (fun (x y : model -> Prop) (m : model) => exists m1 m2 : model, join m1 m2 m /\ x m1 /\ y m2) .
+  Definition logic_equiv := (fun x y : expr => provable (impp x y) /\ provable (impp y x)) .
 End DerivedNames.
 
 Module Type PrimitiveRuleSig (Names: LanguageSig).
@@ -41,8 +42,6 @@ Parameter Inline tree_pos : Type .
   Axiom cancel_mark : (expr_deep -> expr_deep -> tree_pos -> tree_pos -> tree_pos * tree_pos) .
   Axiom cancel_same : (tree_pos -> tree_pos -> Prop) .
   Axiom restore : (tree_pos -> tree_pos -> expr) .
-  Axiom sepcon_assoc1 : (forall x y z : expr, provable (impp (sepcon x (sepcon y z)) (sepcon (sepcon x y) z))) .
-  Axiom sepcon_mono : (forall x1 x2 y1 y2 : expr, provable (impp x1 x2) -> provable (impp y1 y2) -> provable (impp (sepcon x1 y1) (sepcon x2 y2))) .
   Existing Instance sepcon_proper_impp .
 End LogicTheoremSig.
 
@@ -88,8 +87,10 @@ Include Rules.
   Instance minL : (MinimumLanguage L) := (Build_MinimumLanguage L impp) .
   Instance sepconL : (SepconLanguage L) := (Build_SepconLanguage L sepcon) .
   Instance GammaP : (Provable L) := (Build_Provable L provable) .
+  Instance GammaE : (LogicEquiv L) := (Build_LogicEquiv L logic_equiv) .
   Instance J_SA : (SeparationAlgebra model) := (Build_SeparationAlgebra model J join_comm join_assoc) .
   Instance sepconFJ : (SepconDefinition_Join (Pred_sepconL model)) := Join2Sepcon_Normal .
+  Instance GammaEP : (EquivProvable L GammaP GammaE) := Provable2Equiv_Normal .
   Instance sepconAX : (SepconAxiomatization L GammaP) := SeparationAlgebra2SepconAxiomatization .
 Definition tree_pos : Type := tree_pos.
   Definition sepcon_comm_impp : (forall x y : expr, provable (impp (sepcon x y) (sepcon y x))) := sepcon_comm_impp .
@@ -106,8 +107,6 @@ Definition tree_pos : Type := tree_pos.
   Definition cancel_mark : (expr_deep -> expr_deep -> tree_pos -> tree_pos -> tree_pos * tree_pos) := cancel_mark .
   Definition cancel_same : (tree_pos -> tree_pos -> Prop) := cancel_same .
   Definition restore : (tree_pos -> tree_pos -> expr) := restore .
-  Definition sepcon_assoc1 : (forall x y z : expr, provable (impp (sepcon x (sepcon y z)) (sepcon (sepcon x y) z))) := sepcon_assoc1 .
-  Definition sepcon_mono : (forall x1 x2 y1 y2 : expr, provable (impp x1 x2) -> provable (impp y1 y2) -> provable (impp (sepcon x1 y1) (sepcon x2 y2))) := sepcon_mono .
   Existing Instance sepcon_proper_impp .
 End LogicTheorem.
 
